WIP

demo/owned_heap/OHAllocproof.v
@@ -21,6 +21,39 @@ Set Implicit Arguments.
 
 
 Global Opaque string_dec. (**** TODO: Put in SimMem ****)
+(**** TODO: update CoqlibC ****)
+Ltac econsr :=
+  first
+    [ econstructor 30
+     |econstructor 29
+     |econstructor 28
+     |econstructor 27
+     |econstructor 26
+     |econstructor 25
+     |econstructor 24
+     |econstructor 23
+     |econstructor 22
+     |econstructor 21
+     |econstructor 20
+     |econstructor 19
+     |econstructor 18
+     |econstructor 17
+     |econstructor 16
+     |econstructor 15
+     |econstructor 14
+     |econstructor 13
+     |econstructor 12
+     |econstructor 11
+     |econstructor 10
+     |econstructor  9
+     |econstructor  8
+     |econstructor  7
+     |econstructor  6
+     |econstructor  5
+     |econstructor  4
+     |econstructor  3
+     |econstructor  2
+     |econstructor  1].
 
 
 Section SMO.
@@ -36,19 +69,19 @@ Section SMO.
   Inductive wf (smo: t): Prop :=
   | wf_intro
       (MWF: SimMem.wf smo)
-      (map: block -> option int) (u: unit)
+      (map: block -> option int)
       (OHSRC: smo.(oh_src) = upcast map)
-      (OHTGT: smo.(oh_tgt) = upcast u)
+      (OHTGT: smo.(oh_tgt) = upcast tt)
       (SOME: forall
           k v
           (SOME: map k = Some v)
         ,
           (* (<<SRC: forall o, ZMap.get o (smo.(SimMem.src).(Mem.mem_contents) # k) = Undef>>) /\ *)
-          (<<SRC: Mem_range_noperm smo.(SimMem.src) k 0%Z 4%Z>>) /\
+          (<<SRC: Mem_range_noperm smo.(SimMem.src) k lo hi>>) /\
           (* (<<SRC: (smo.(SimMem.tgt).(Mem.mem_contents) # k) = (ZMap.init Undef)>>) /\ *)
           (<<TGT: Mem.load Mint32 smo.(SimMem.tgt) k 0%Z = Some (Vint v)>>) /\
-          (<<PMSRC: brange k 0 4 <2= privmods (Some "OHAlloc") smo.(sm).(SimMem.ptt_src)>>) /\
-          (<<PMTGT: brange k 0 4 <2= privmods (Some "OHAlloc") smo.(sm).(SimMem.ptt_tgt)>>) /\
+          (<<PMSRC: brange k lo hi <2= privmods (Some "OHAlloc") smo.(sm).(SimMem.ptt_src)>>) /\
+          (<<PMTGT: brange k lo hi <2= privmods (Some "OHAlloc") smo.(sm).(SimMem.ptt_tgt)>>) /\
           (<<VLSRC: Mem.valid_block smo.(SimMem.src) k>>)
       )
   .
@@ -87,7 +120,7 @@ Section SMO.
     econs; ss; et.
     ii. exploit SOME; et. i; des. esplits; ss; et.
     - eapply Mem_unchanged_noperm; et.
-    - eapply Mem.load_unchanged_on; et. ii. ss. eapply PMTGT0; et.
+    - eapply Mem.load_unchanged_on; et. ii. ss. eapply PMTGT0; et. rr. unfold lo, hi. esplits; et; xomega.
     - eapply Mem.valid_block_unchanged_on; et.
   Qed.
   Next Obligation.
@@ -113,715 +146,184 @@ Let tge := Build_genv (SkEnv.revive (SkEnv.project skenv_link (Mod.sk md_tgt)) p
 Definition msp: ModSemPair.t :=
   ModSemPair.mk (md_src skenv_link) (md_tgt skenv_link) (SimSymbId.mk md_src md_tgt) sm_link SimMemOh.
 
-Inductive match_states_internal: nat -> MutrecAspec.state -> Clight.state -> Prop :=
-| match_callstate_nonzero
-    idx i m_src m_tgt
-    fptr
-    (RANGE: 0 <= i.(Int.intval) < MAX)
-    (FINDF: Genv.find_funct (Smallstep.globalenv (modsem2 skenv_link prog)) fptr = Some (Internal func_f))
-    (IDX: (idx > 3)%nat)
+Local Existing Instance SimMemOh.
+
+Inductive match_states: nat -> OHAllocSource.state -> Clight.state -> SimMemOh.t -> Prop :=
+| match_callstate_new
+    oh m_src m_tgt fptr_tgt tyf vs_tgt (smo0: SimMemOh.t)
+    (MWF: SimMemOh.wf smo0)
+    (OH: smo0.(oh_src) = upcast oh)
+    (MSRC: m_src = smo0.(SimMem.src))
+    (MTGT: m_tgt = smo0.(SimMem.tgt))
+    (FINDF: Genv.find_funct tge fptr_tgt = Some (Internal (f_new)))
+    (TYF: tyf = (Clight.type_of_function f_new))
+    (VSTGT: vs_tgt = [])
   :
-    match_states_internal idx (Callstate i m_src) (Clight.Callstate fptr (Tfunction
-                                                                            (Tcons tint Tnil) tint cc_default)
-                                                                    [Vint i] Kstop m_tgt)
-| match_returnstate
-    idx i m_src m_tgt
+    match_states 0%nat
+                 (CallstateNew oh m_src)
+                 (Callstate fptr_tgt tyf vs_tgt Kstop m_tgt)
+                 smo0
+| match_callstate_get
+    oh m_src m_tgt fptr_tgt tyf vs_tgt (smo0: SimMemOh.t)
+    blk_src
+    (MWF: SimMemOh.wf smo0)
+    (OH: smo0.(oh_src) = upcast oh)
+    (MSRC: m_src = smo0.(SimMem.src))
+    (MTGT: m_tgt = smo0.(SimMem.tgt))
+    (FINDF: Genv.find_funct tge fptr_tgt = Some (Internal (f_get)))
+    (TYF: tyf = (Clight.type_of_function f_get))
+    (SIMVS: SimMem.sim_val_list smo0 [Vptr blk_src Ptrofs.zero] vs_tgt)
   :
-    match_states_internal idx (Returnstate i m_src) (Clight.Returnstate (Vint i) Kstop m_tgt)
+    match_states 0%nat
+                 (CallstateGet blk_src oh m_src)
+                 (Callstate fptr_tgt tyf vs_tgt Kstop m_tgt)
+                 smo0
+| match_callstate_set
+    oh m_src m_tgt fptr_tgt tyf vs_tgt (smo0: SimMemOh.t)
+    blk_src v_src
+    (MWF: SimMemOh.wf smo0)
+    (OH: smo0.(oh_src) = upcast oh)
+    (MSRC: m_src = smo0.(SimMem.src))
+    (MTGT: m_tgt = smo0.(SimMem.tgt))
+    (FINDF: Genv.find_funct tge fptr_tgt = Some (Internal (f_set)))
+    (TYF: tyf = (Clight.type_of_function f_set))
+    (SIMVS: SimMem.sim_val_list smo0 [Vptr blk_src Ptrofs.zero ; Vint v_src] vs_tgt)
+  :
+    match_states 0%nat
+                 (CallstateSet blk_src v_src oh m_src)
+                 (Callstate fptr_tgt tyf vs_tgt Kstop m_tgt)
+                 smo0
+| match_returnstate_new
+    oh m_src m_tgt blk_src v_tgt (smo0: SimMemOh.t)
+    (MWF: SimMemOh.wf smo0)
+    (OH: smo0.(oh_src) = upcast oh)
+    (MSRC: m_src = smo0.(SimMem.src))
+    (MTGT: m_tgt = smo0.(SimMem.tgt))
+    (SIMVAL: SimMem.sim_val smo0 (Vptr blk_src Ptrofs.zero) v_tgt)
+  :
+    match_states 0%nat
+                 (ReturnstateNew blk_src oh m_src)
+                 (Returnstate v_tgt Kstop m_tgt)
+                 smo0
 .
 
-
-
-Inductive match_states
-          (idx: nat) (st_src0: MutrecAspec.state) (st_tgt0: Clight.state) (sm0: SimMem.t): Prop :=
-| match_states_intro
-    (MATCHST: match_states_internal idx st_src0 st_tgt0)
-    (MCOMPATSRC: (get_mem st_src0) = sm0.(SimMem.src))
-    (MCOMPATTGT: (ClightC.get_mem st_tgt0) = sm0.(SimMem.tgt))
-    (MWF: SimMem.wf sm0)
-.
-
-Lemma g_blk_exists
-  :
-    exists g_blk,
-      (<<FINDG: Genv.find_symbol
-                  (SkEnv.revive (SkEnv.project skenv_link (CSk.of_program signature_of_function prog)) prog)
-                  g_id = Some g_blk>>)
-      /\
-      (<<FINDG: Genv.find_funct_ptr
-                  (SkEnv.revive (SkEnv.project skenv_link (CSk.of_program signature_of_function prog)) prog)
-                  g_blk = None>>)
-      /\
-      (<<FINDG: exists skd, Genv.find_funct_ptr skenv_link g_blk = Some skd /\
-                            Some (signature_of_type (Tcons tint Tnil) tint cc_default) = Sk.get_csig skd>>)
-.
+Theorem sim_modsem: ModSemPair.sim msp.
 Proof.
-  exploit (prog_defmap_norepet prog g_id); eauto.
-  { unfold prog_defs_names. ss. repeat (econs; eauto).
-    - ii; ss; des; ss.
-    - ii; ss; des; ss. }
-  { ss. eauto. }
-  intro T; des.
-  exploit SkEnv.project_impl_spec; eauto. intro PROJ.
-  assert(PREC: SkEnv.genv_precise
-                 (SkEnv.revive (SkEnv.project skenv_link (CSk.of_program signature_of_function prog)) prog)
-                 prog).
-  { eapply CSkEnv.project_revive_precise; ss; et. }
-  inv PREC.
-  exploit (P2GE g_id); eauto. i; des. des_ifs.
-  rename b into g_blk.
-  eexists. splits; et.
-  { unfold Genv.find_funct_ptr. des_ifs. }
-  { inv INCL.
-    exploit (CSk.of_program_prog_defmap prog signature_of_function); et. rewrite T. intro S.
+  eapply match_states_sim with
+      (match_states := match_states) (match_states_at := bot4)
+      (has_footprint := top3) (mle_excl := fun _ _ => SimMemOh.le) (sidx := unit);
+    eauto; ii; ss; folder.
+  - eapply lt_wf.
+  - eapply SoundTop.sound_state_local_preservation; et.
+  - r. etrans; et.
+  - des. inv INITTGT. folder. ss.
+    inv SAFESRC.
+    + destruct args_src; ss. clarify.
+      rr in SIMARGS; des. inv SIMARGS0; ss. clarify. folder.
+      esplits; try refl.
+      { econs; et. }
+      assert(T: Genv.find_funct tge fptr_tgt = Some (Internal f_new)).
+      { admit "FINDF". }
+      ss. clarify.
+      econs; et.
+      inv VALS; ss. inv TYP; ss.
+    + admit "NOT NOW".
+    + admit "NOT NOW".
+  - des. rr in SIMARGS; des. inv SAFESRC; inv SIMARGS0; ss; clarify.
+    + assert(T: Genv.find_funct (SkEnv.revive ge prog) fptr_tgt = Some (Internal (f_new))).
+      { admit "FINDF". }
+      inv VALS.
+      esplits; et. econs; et. ss.
+    + admit "NOT NOW".
+    + admit "NOT NOW".
+  - inv MATCH; ss.
+  - inv FINALSRC; inv MATCH; ss.
+    + esplits; et.
+      * econs; et.
+      * rr. esplits; ss; et.
+        { econs; et. }
+        instantiate (1:= tt). inv MWF. ss.
+      * refl.
+      * refl.
+  - left.
+    esplits; et.
+    { admit "receptive". }
+    ii. inv MATCH; inv STEPSRC; ss.
+    + exploit SimMemSV.alloc_parallel; try apply ALLOC; try refl.
+      { eapply MWF. }
+      i; des. clarify.
+      exploit SimMemSV.free_left; et. i; des. clarify.
 
-    remember ((prog_defmap (CSk.of_program signature_of_function prog)) ! g_id) as U in *.
-    destruct U eqn:V; try (by ss). inv S. inv H1.
 
-    exploit DEFS; eauto. i; des.
-    assert(blk = g_blk).
-    { inv PROJ. exploit SYMBKEEP; et.
-      - instantiate (1:= g_id). unfold defs. des_sumbool. ss. et.
-      - i. rewrite SYMB0 in *. clear - SYMB H. unfold SkEnv.revive in *. rewrite Genv_map_defs_symb in *. ss.
-        rewrite SYMB in *. des. clarify.
-    }
-    clarify. inv MATCH.
-    esplits; eauto.
-    - unfold Genv.find_funct_ptr. rewrite DEF0. et.
-    - ss. des_ifs. clear - H1. inv H1; ss.
-  }
-Qed.
 
-Lemma match_states_lxsim
-      idx st_src0 st_tgt0 sm0
-      (SIMSK: SimSymb.sim_skenv
-                sm0 (SimMemInjInvC.mk symbol_memoized md_src md_tgt)
-                (SkEnv.project skenv_link (CSk.of_program signature_of_function prog))
-                (SkEnv.project skenv_link (CSk.of_program signature_of_function prog)))
-      (MATCH: match_states idx st_src0 st_tgt0 sm0)
-  :
-    <<XSIM: lxsimL (md_src skenv_link) (md_tgt skenv_link)
-                   (fun st => unit -> exists su m_init, SoundTop.sound_state su m_init st)
-                   top3 (fun _ _ => SimMem.le)
-                   (Ord.lift_idx lt_wf idx) st_src0 st_tgt0 sm0>>
-.
-Proof.
-  revert_until tge.
-  pcofix CIH.
-  i.
-  pfold.
-  generalize g_blk_exists; et. i; des.
-  inv MATCH; subst. ss. inv MATCHST; ss; clarify.
-  - (* call *)
-    destruct (classic (i = Int.zero)).
-    + (* zero *)
-      clarify.
-      econs 2. ii.
-      econs 2; et.
-      { split.
-        - econs 2.
-          + ss. econs 1.
-          + econs 1.
-          + ss.
-        - eapply Ord.lift_idx_spec.
-          instantiate (1:=3%nat). nia. }
-      refl.
 
-      left. pfold.
-      econs 1. i; des.
-      econs 2; et.
-
-      * split; cycle 1.
-        { apply Ord.lift_idx_spec.
-          instantiate (1:=2%nat). nia. }
-
+      eexists _, _, _, (mk (SimMemSV.mk _ _ _ _ _ _ _) _ _); ss. esplits; et.
+      { apply star_refl. }
+      { left.
+        eapply ModSemProps.spread_dplus; et.
+        { admit "determinate". }
         eapply plus_left with (t1 := E0) (t2 := E0); ss.
         { econs; eauto.
-          { eapply modsem2_determinate; eauto. }
-          econs; eauto.
           econs; ss; eauto; try (by repeat (econs; ss; eauto)).
-          unfold _x. unfold _t'1. rr. ii; ss. des; ss; clarify.
         }
-
         eapply star_left with (t1 := E0) (t2 := E0); ss.
-        { econs; eauto.
-          { eapply modsem2_determinate; eauto. }
-          econs; eauto.
-        }
-
+        { econs; et. }
         eapply star_left with (t1 := E0) (t2 := E0); ss.
-        { econs; eauto.
-          { eapply modsem2_determinate; eauto. }
-          econs; eauto.
+        { econs; et. }
+        eapply star_left with (t1 := E0) (t2 := E0); ss.
+        { econs; ss; et.
+          (** TODO: we might need better "econs" tactic for multiple choices **)
+          - econs; et.
+            { repeat econsr; et. folder. admit "FINDF". }
+            { econs 2; ss; et. }
           - repeat econs; et.
-          - ss.
         }
-
         eapply star_left with (t1 := E0) (t2 := E0); ss.
-        { econs; eauto.
-          { eapply modsem2_determinate; eauto. }
-          econs; eauto.
-          - repeat econs; et.
-          - ss.
-          - ss.
+        { econsr; ss; et.
+          - folder. des_ifs. instantiate (1:= EF_malloc).
+            admit "FINDF".
+          - rr. econs; ss; et. unfold Mptr; des_ifs; ss. psimpl.
+            admit "store_right".
         }
-
+        eapply star_left with (t1 := E0) (t2 := E0); ss.
+        { econs; ss; et. }
+        eapply star_left with (t1 := E0) (t2 := E0); ss.
+        { econs; ss; et. }
+        eapply star_left with (t1 := E0) (t2 := E0); ss.
+        { econs; ss; et.
+          econs; ss; et.
+        }
+        eapply star_left with (t1 := E0) (t2 := E0); ss.
+        { econs; ss; et. }
+        eapply star_left with (t1 := E0) (t2 := E0); ss.
+        { econs; ss; et. }
+        eapply star_left with (t1 := E0) (t2 := E0); ss.
+        { repeat (econs; ss; et).
+          admit "store_right".
+        }
+        eapply star_left with (t1 := E0) (t2 := E0); ss.
+        { econs; ss; et. }
+        eapply star_left with (t1 := E0) (t2 := E0); ss.
+        { repeat econs; ss; et. }
         apply star_refl.
-      * refl.
-      * right. eapply CIH; eauto. econs; ss; eauto.
-        replace (Int.repr 0) with (sum Int.zero).
-        { econs; eauto. }
-        { rewrite sum_recurse. des_ifs. }
-
-    + (* nonzero *)
-
-      destruct (Genv.find_symbol
-                  (SkEnv.project skenv_link (CSk.of_program signature_of_function prog))
-                  _memoized) eqn:BLK; cycle 1.
-      { exfalso. clear - INCL BLK. inversion INCL; subst.
-        exploit DEFS; eauto.
-        - instantiate (2:=_memoized). ss.
-        - i. des.
-          exploit SkEnv.project_impl_spec. eapply INCL. i. inv H. ss.
-          exploit SYMBKEEP. instantiate (1:=_memoized). ss. i.
-          rr in H. rewrite H in *. clarify. }
-
-      inv MWF. ss.
-
-      assert (INVAR: SimMemInjInv.mem_inv_tgt sm0 b).
-      { inv SIMSK. ss. inv INJECT.
-        eapply INVCOMPAT; eauto. ss. }
-
-      hexploit SATTGT; eauto. intros SAT0.
-      exploit SAT0; eauto. i. inv H0. ss.
-      hexploit LOADVALS; eauto. i. des.
-
-      destruct (zeq (Int.intval i0) 0).
+      }
       {
-        econs 2. ii.
-        econs 2; et.
-        { split.
-          - econs 2; ss.
-            + econs 2; eauto.
-              clear - H.
-              exploit Int.eq_false; eauto. i.
-              unfold Int.eq in *. ss. des_ifs.
-            + econs; eauto.
-            + ss.
-          - eapply Ord.lift_idx_spec. eauto. }
-        refl.
-
-        left. pfold.
-        econs.
-        i; des.
-        econs 2; eauto.
-        * esplits; cycle 1.
-          { eapply Ord.lift_idx_spec. eauto. }
-
-          eapply plus_left with (t1 := E0) (t2 := E0); ss.
-          { econs; eauto.
-            { eapply modsem2_determinate; eauto. }
-            econs; eauto.
-            econs; ss; eauto; try (by repeat (econs; ss; eauto)).
-            unfold _x. unfold _t'1. rr. ii; ss. des; ss; clarify.
-          }
-
-          eapply star_left with (t1 := E0) (t2 := E0); ss.
-          { econs; eauto.
-            { eapply modsem2_determinate; eauto. }
-            econs; eauto.
-          }
-
-          eapply star_left with (t1 := E0) (t2 := E0); ss.
-          { econs; eauto.
-            { eapply modsem2_determinate; eauto. }
-            econs; eauto.
-            - repeat econs; et.
-            - ss. rewrite Int.eq_false; ss.
-          }
-
-          eapply star_left with (t1 := E0) (t2 := E0); ss.
-          { econs; eauto.
-            { eapply modsem2_determinate; eauto. }
-            econs; eauto.
-          }
-
-          eapply star_left with (t1 := E0) (t2 := E0); ss.
-          { econs; eauto.
-            { eapply modsem2_determinate; eauto. }
-            econs; eauto.
-          }
-
-          eapply star_left with (t1 := E0) (t2 := E0); ss.
-          { econs; eauto.
-            { eapply modsem2_determinate; eauto. }
-            econs; eauto; swap 1 2.
-            - econs.
-              + ss. econs. econs; ss.
-                * econs.
-                  { eapply eval_Evar_global; ss.
-                    instantiate (1:=b). eauto. }
-                  { econs 2; ss. }
-                * econs; ss.
-                * ss.
-              + econs 1; ss. psimpl.
-                replace (Ptrofs.unsigned (Ptrofs.mul (Ptrofs.repr 4) (Ptrofs.of_ints i)))
-                  with (4 * Int.intval i); cycle 1.
-                { unfold Ptrofs.mul. ss.
-                  destruct i. ss. unfold Ptrofs.of_ints. ss.
-                  unfold Int.signed. ss. des_ifs; cycle 1;
-                  unfold Int.half_modulus, Int.modulus, two_power_nat in *; ss;
-                    unfold MAX in *; rewrite <- Zdiv2_div in *; ss.
-                  { lia. }
-                  repeat rewrite Ptrofs.unsigned_repr. auto.
-                  all : unfold Ptrofs.max_unsigned; rewrite Ptrofs.modulus_power;
-                  unfold Ptrofs.zwordsize, Ptrofs.wordsize, Wordsize_Ptrofs.wordsize; des_ifs; ss; omega. } eauto. }
-
-          eapply star_left with (t1 := E0) (t2 := E0); ss.
-          { econs; eauto.
-            { eapply modsem2_determinate; eauto. }
-            econs; eauto.
-          }
-
-          eapply star_left with (t1 := E0) (t2 := E0); ss.
-          { econs; eauto.
-            { eapply modsem2_determinate; eauto. }
-            econs; eauto.
-          }
-
-          eapply star_left with (t1 := E0) (t2 := E0); ss.
-          { econs; eauto.
-            { eapply modsem2_determinate; eauto. }
-            ss. econs; eauto.
-            - econs; ss.
-              + econs; ss.
-              + econs; ss.
-              + ss.
-            - ss. instantiate (1:=true).
-              unfold Cop.bool_val. ss.
-              unfold Int.eq. unfold Val.of_bool.
-              destruct (zeq (Int.unsigned i0) (Int.unsigned (Int.repr 0))) eqn:EQ; ss. }
-          eapply star_left with (t1 := E0) (t2 := E0); ss.
-          { econs; eauto.
-            { eapply modsem2_determinate; eauto. }
-            econs; eauto.
-          }
-
-          eapply star_left with (t1 := E0) (t2 := E0); ss.
-          { econs; eauto.
-            { eapply modsem2_determinate; eauto. }
-            econs; eauto.
-          }
-
-          eapply star_left with (t1 := E0) (t2 := E0); ss.
-          { econs; eauto.
-            { eapply modsem2_determinate; eauto. }
-            econs; eauto; swap 1 2.
-            - econs.
-              + eapply eval_Evar_global; ss. et.
-              + econs 2; et.
-            - unfold Cop.classify_fun. ss.
-            - repeat econs; ss; et.
-          }
-
-          eapply star_refl.
-
-        * refl.
-
-        * left. pfold. econs 3; et.
-          { econs; eauto. }
-          { rr. esplits; et. econs; eauto. }
-          ii; des.
-          inv ATSRC. ss; clarify.
-
-          unfold Clight.fundef in *.
-          assert(g_fptr = g_blk).
-          { unfold SkEnv.revive in FINDG. rewrite Genv_map_defs_symb in *. clarify. }
-          clarify.
-          eexists tt, (Args.mk _ [Vint (Int.sub i (Int.repr 1))] _).
-          exists sm0.
-          esplits; ss; eauto.
-          { rr. esplits; ss; et. econs; ss; eauto.
-            instantiate (1:=Vptr g_blk Ptrofs.zero).
-            inv SIMSK. inv SIMSKENV. inv INJECT. ss.
-            econs. eapply DOMAIN; eauto.
-            exploit Genv.genv_symb_range. unfold Genv.find_symbol in *. eauto.
-            i. ss. ii.
-            exploit INVCOMPAT; eauto. i. rewrite <- H1 in H0. ss.
-            rewrite Ptrofs.add_zero_l. ss. }
-          { refl. }
-          { econs; eauto. }
-          i. inv AFTERSRC. rr in SIMRETV; des. inv SIMRETV0; ss; clarify.
-
-          hexploit Mem.valid_access_store.
-          { instantiate (4:=sm_ret.(SimMemInjInv.minj).(SimMemInj.tgt)).
-            inv MWF. inv WF. exploit SATTGT0; eauto.
-            - inv MLE. erewrite <- MINVEQTGT. eauto.
-            - i. inv H0. hexploit PERMISSIONS0; eauto. ss.
-              esplits; eauto. }
-          intros [m_tgt STR].
-
-          exploit SimMemInjInvC.unlift_wf; try apply MLE; eauto.
-          { econs; eauto. } intros MLE1.
-          exploit memoized_inv_store_le; eauto.
-          i. des.
-
-          esplits.
-          { econs; eauto. }
-          { apply MLE0. }
-          { et. }
-
-          left. pfold. econs; eauto. i; des. econs 2; eauto.
-          {
-            esplits; eauto; cycle 1.
-            { instantiate (1:= (Ord.lift_idx lt_wf 14%nat)). eapply Ord.lift_idx_spec; et. }
-
-            eapply plus_left with (t1 := E0) (t2 := E0); ss.
-            { econs; eauto.
-              { eapply modsem2_determinate; eauto. }
-              econs; eauto.
-            }
-
-            eapply star_left with (t1 := E0) (t2 := E0); ss.
-            { econs; eauto.
-              { eapply modsem2_determinate; eauto. }
-              econs; eauto.
-            }
-
-            eapply star_left with (t1 := E0) (t2 := E0); ss.
-            { econs; eauto.
-              { eapply modsem2_determinate; eauto. }
-              econs; eauto. econs; eauto.
-              - econs; eauto. ss.
-              - econs; eauto. ss.
-              - inv RETV. ss. unfold typify. des_ifs. }
-
-            eapply star_left with (t1 := E0) (t2 := E0); ss.
-            { econs; eauto.
-              { eapply modsem2_determinate; eauto. }
-              econs; eauto.
-            }
-
-            eapply star_left with (t1 := E0) (t2 := E0); ss.
-            { econs; eauto.
-              { eapply modsem2_determinate; eauto. }
-              econs; eauto.
-              - econs; eauto. econs; eauto.
-                + econs; eauto.
-                  * eapply eval_Evar_global; ss.
-                    instantiate (1:=b). ss.
-                  * ss. econs 2; eauto.
-                + econs; eauto. ss.
-                + econs; eauto.
-              - econs; eauto. ss.
-              - ss.
-              - ss. psimpl. econs; ss; eauto.
-                rpapply STR. f_equal.
-                + unfold Ptrofs.mul. ss.
-                  destruct i. ss. unfold Ptrofs.of_ints. ss.
-                  unfold Int.signed. ss. des_ifs; cycle 1;
-                  unfold Int.half_modulus, Int.modulus, two_power_nat in *; ss;
-                    unfold MAX in *; rewrite <- Zdiv2_div in *; ss.
-                  { lia. }
-                  repeat rewrite Ptrofs.unsigned_repr. auto.
-                  all : unfold Ptrofs.max_unsigned; rewrite Ptrofs.modulus_power;
-                    unfold Ptrofs.zwordsize, Ptrofs.wordsize, Wordsize_Ptrofs.wordsize; des_ifs; ss; omega.
-                + f_equal.
-                  rewrite Int.repr_unsigned.
-                  rewrite sum_recurse with (i := i). des_ifs.
-                  rewrite Z.eqb_eq in Heq.
-                  exploit Int.eq_spec. instantiate (1:=i). instantiate (1:=Int.zero).
-                  unfold Int.eq. unfold Int.unsigned. rewrite Heq. des_ifs. i. subst i.
-                  rewrite Int.sub_zero_r. rewrite sum_recurse. des_ifs. }
-
-            eapply star_left with (t1 := E0) (t2 := E0); ss.
-            { econs; eauto.
-              { eapply modsem2_determinate; eauto. }
-              econs; eauto.
-            }
-
-            eapply star_left with (t1 := E0) (t2 := E0); ss.
-            { econs; eauto.
-              { eapply modsem2_determinate; eauto. }
-              econs; eauto.
-              - econs; eauto. ss.
-              - econs; eauto.
-              - econs; eauto. }
-
-            eapply star_refl.
-          }
-          { refl. }
-
-          right. eapply CIH.
-          { eapply SimMemInjInvC.sim_skenv_inj_lepriv; cycle 1; eauto.
-            etrans; eauto.
-            { exploit (SimMemLift.lift_priv sm0); eauto. ss. }
-            etrans; eauto; cycle 1.
-            { hexploit SimMem.pub_priv; try apply MLE0. eauto. }
-            etrans; eauto.
-            { hexploit SimMem.pub_priv; try apply MLE; eauto. }
-            hexploit SimMemLift.unlift_priv; revgoals.
-            { intro T. ss. eauto. }
-            { eauto. }
-            { eauto. }
-            { exploit (SimMemLift.lift_priv sm0); eauto. ss. }
-            { econs; eauto. } }
-          { econs; ss.
-            - replace (Int.add (sum (Int.sub i Int.one)) i) with (sum i); cycle 1.
-              { rewrite sum_recurse with (i := i). des_ifs.
-                rewrite Z.eqb_eq in Heq.
-                exploit Int.eq_spec. instantiate (1:=i). instantiate (1:=Int.zero).
-                unfold Int.eq. unfold Int.unsigned. rewrite Heq. des_ifs. i. subst i.
-                rewrite Int.sub_zero_r. rewrite sum_recurse. des_ifs. }
-
-              econs 2.
-          }
+        admit "le".
       }
-
-      { hexploit VAL; eauto. i. des. clarify.
-
-        econs 2. ii.
-        econs 2; et.
-        { split.
-          - econs 2; ss.
-            + econs; eauto.
-            + econs; eauto.
-            + ss.
-          - eapply Ord.lift_idx_spec. eauto. }
-        refl.
-
-        left. pfold.
-        econs.
-        i; des.
-        econs 2; eauto.
-        * esplits; cycle 1.
-          { eapply Ord.lift_idx_spec. eauto. }
-
-          eapply plus_left with (t1 := E0) (t2 := E0); ss.
-          { econs; eauto.
-            { eapply modsem2_determinate; eauto. }
-            econs; eauto.
-            econs; ss; eauto; try (by repeat (econs; ss; eauto)).
-            unfold _x. unfold _t'1. rr. ii; ss. des; ss; clarify.
-          }
-
-          eapply star_left with (t1 := E0) (t2 := E0); ss.
-          { econs; eauto.
-            { eapply modsem2_determinate; eauto. }
-            econs; eauto.
-          }
-
-          eapply star_left with (t1 := E0) (t2 := E0); ss.
-          { econs; eauto.
-            { eapply modsem2_determinate; eauto. }
-            econs; eauto.
-            - repeat econs; et.
-            - ss. rewrite Int.eq_false; ss.
-          }
-
-          eapply star_left with (t1 := E0) (t2 := E0); ss.
-          { econs; eauto.
-            { eapply modsem2_determinate; eauto. }
-            econs; eauto.
-          }
-
-          eapply star_left with (t1 := E0) (t2 := E0); ss.
-          { econs; eauto.
-            { eapply modsem2_determinate; eauto. }
-            econs; eauto.
-          }
-
-          eapply star_left with (t1 := E0) (t2 := E0); ss.
-          { econs; eauto.
-            { eapply modsem2_determinate; eauto. }
-            econs; eauto; swap 1 2.
-            - econs.
-              + ss. econs. econs; ss.
-                * econs.
-                  { eapply eval_Evar_global; ss.
-                    instantiate (1:=b). ss. }
-                  { econs 2; ss. }
-                * econs; ss.
-                * ss.
-              + econs 1; ss. psimpl.
-                replace (Ptrofs.unsigned (Ptrofs.mul (Ptrofs.repr 4) (Ptrofs.of_ints i)))
-                  with (4 * Int.intval i); cycle 1.
-                { unfold Ptrofs.mul. ss.
-                  destruct i. ss. unfold Ptrofs.of_ints. ss.
-                  unfold Int.signed. ss. des_ifs; cycle 1;
-                  unfold Int.half_modulus, Int.modulus, two_power_nat in *; ss;
-                    unfold MAX in *; rewrite <- Zdiv2_div in *; ss.
-                  { lia. }
-                  repeat rewrite Ptrofs.unsigned_repr. auto.
-                  all : unfold Ptrofs.max_unsigned; rewrite Ptrofs.modulus_power;
-                  unfold Ptrofs.zwordsize, Ptrofs.wordsize, Wordsize_Ptrofs.wordsize; des_ifs; ss; omega. } eauto. }
-
-          eapply star_left with (t1 := E0) (t2 := E0); ss.
-          { econs; eauto.
-            { eapply modsem2_determinate; eauto. }
-            econs; eauto.
-          }
-
-          eapply star_left with (t1 := E0) (t2 := E0); ss.
-          { econs; eauto.
-            { eapply modsem2_determinate; eauto. }
-            econs; eauto.
-          }
-
-          eapply star_left with (t1 := E0) (t2 := E0); ss.
-          { econs; eauto.
-            { eapply modsem2_determinate; eauto. }
-            ss. econs; eauto.
-            - econs; ss.
-              + econs; ss.
-              + econs; ss.
-              + ss.
-            - ss. instantiate (1:=false).
-              unfold Cop.bool_val. ss.
-              unfold Int.eq. unfold Val.of_bool.
-              destruct (zeq (Int.unsigned (sum (Int.repr (Int.intval i))))
-                            (Int.unsigned (Int.repr 0))) eqn:EQ; ss. }
-
-          eapply star_left with (t1 := E0) (t2 := E0); ss.
-          { econs; eauto.
-            { eapply modsem2_determinate; eauto. }
-            econs; eauto.
-          }
-
-          eapply star_left with (t1 := E0) (t2 := E0); ss.
-          { econs; eauto.
-            { eapply modsem2_determinate; eauto. }
-            econs; eauto.
-            - econs; ss.
-            - econs.
-            - ss. }
-
-          apply star_refl.
-
-        * refl.
-
-        * right. eapply CIH; eauto.
-          { econs; eauto.
-            - ss. replace (Int.repr (Int.intval i)) with i.
-              + econs; eauto.
-              + symmetry. eapply Int.eqm_repr_eq.
-                eapply Int.eqm_refl2. ss.
-            - econs; eauto. }
+      {
+        admit "unch".
       }
-
-  - (* return *)
-    econs 4; ss; eauto.
-    + refl.
-    + rr. esplits; ss; et. econs; ss; eauto.
+      {
+        econs 4 ; ss; et.
+        admit "wf".
+      }
+    + admit "NOTNOW".
+    + admit "NOTNOW".
+  - eexists (mk sm0 _ _); ss. esplits; et. econs; ss; et.
 Unshelve.
   all: ss.
+  all: admit "NOTNOW".
 Qed.
-
-Theorem sim_modsem
-  :
-    ModSemPair.sim msp
-.
-Proof.
-  eapply sim_mod_sem_implies.
-  eapply ModSemPair.simL_intro with (has_footprint := top3) (mle_excl := fun _ _ => SimMem.le); try (by ss).
-  { i. eapply SoundTop.sound_state_local_preservation. }
-  { i. eapply Preservation.local_preservation_noguarantee_weak; eauto. eapply SoundTop.sound_state_local_preservation. }
-  { ii; ss. r. etrans; eauto. }
-  { ii. eauto. }
-  { esplits; et. }
-  i. ss. esplits; eauto.
-
-  - i. des. inv SAFESRC.
-    esplits; eauto.
-    + refl.
-    + eapply SimMemInjInvC.unch_true; et.
-    + econs; eauto.
-    + instantiate (1:= (Ord.lift_idx lt_wf 15%nat)).
-      inv INITTGT. inv TYP. ss.
-      assert (FD: fd = func_f).
-      { destruct args_src, args_tgt; ss. clarify.
-        rr in SIMARGS; des. inv SIMARGS0; ss. clarify. inv VALS. inv H1. inv H3. inv FPTR. ss.
-        des_ifs.
-        inv SIMSKENV. ss. inv SIMSKE. ss. inv INJECT. ss.
-        exploit IMAGE; eauto.
-        { exploit Genv.genv_symb_range.
-          unfold Genv.find_symbol in SYMB. eauto. i. ss. eauto. }
-        ii. des. subst. clarify.
-
-        rewrite Genv.find_funct_ptr_iff in FINDF.
-        unfold Genv.find_def in FINDF. ss.
-        do 2 rewrite MapsC.PTree_filter_map_spec, o_bind_ignore in *.
-        des_ifs.
-        destruct (Genv.invert_symbol
-                    (SkEnv.project skenv_link (CSk.of_program signature_of_function prog)) b2) eqn:SKENVSYMB; ss.
-        unfold o_bind in FINDF. ss.
-        exploit Genv.find_invert_symbol. eauto. i.
-        rewrite H in *. clarify.
-        destruct ((prog_defmap prog) ! f_id) eqn:DMAP; ss. clarify. } clarify.
-
-      rr in SIMARGS; des. inv SIMARGS0; ss. clarify. inv VALS.
-      inv H3. inv H1.
-      unfold typify_list, zip, typify. ss. des_ifs; ss.
-
-      eapply match_states_lxsim; ss.
-      * inv SIMSKENV; eauto.
-      * econs; eauto.
-        { econs; eauto. omega. }
-
-  - (* init progress *)
-    i.
-    des. inv SAFESRC.
-    rr in SIMARGS; des. inv SIMARGS0; ss. clarify.
-
-    esplits; eauto. econs; eauto.
-    + instantiate (1:= func_f).
-      ss.
-      inv VALS; ss. inv H1. inv H3. inv FPTR0. ss.
-      des_ifs.
-      inv SIMSKENV. ss. inv SIMSKE. ss. inv INJECT. ss.
-      exploit IMAGE; eauto.
-      { exploit Genv.genv_symb_range.
-        unfold Genv.find_symbol in SYMB. eauto. i. ss. eauto. }
-      ii. des. subst. clarify.
-
-      rewrite Genv.find_funct_ptr_iff in *.
-      unfold Genv.find_def in *; ss.
-      do 2 rewrite MapsC.PTree_filter_map_spec, o_bind_ignore in *.
-      des_ifs.
-      exploit Genv.find_invert_symbol. eauto. i.
-      rewrite H in *. clarify.
-    + econs; ss. erewrite <- inject_list_length; eauto.
-      auto.
-Qed.
-
 
 End SIMMODSEM.
 
-
-Theorem sim_mod
-  :
-    ModPair.sim (ModPair.mk (MutrecAspec.module) (ClightC.module2 prog) (SimMemInjInvC.mk symbol_memoized (MutrecAspec.module) (ClightC.module2 prog)))
-.
-Proof.
-  econs; ss.
-  - econs; ss.
-    + i. inv SS. esplits; ss; eauto.
-      * econs; ss.
-        ii. des. econs.
-        { ii. ss. des. clarify. econs; ss.
-          - ii. eapply PERM; eauto. unfold MAX in *. lia.
-          - eapply Z.divide_factor_l. }
-        { ss. i. clarify. erewrite INIT; ss; eauto.
-          - esplits; eauto. i. rewrite sum_recurse. des_ifs.
-          - lia.
-          - unfold MAX. lia.
-          - eapply Z.divide_factor_l. }
-      * ii. des; clarify.
-    + ii. destruct H. eapply in_prog_defmap in PROG.
-      ss. unfold update_snd in PROG. ss.
-      des; clarify; inv DROP; ss.
-      des; clarify.
-  - ii. ss.
-    inv SIMSKENVLINK. inv SIMSKENV.
-    eexists. eapply sim_modsem; eauto.
-Qed.
